isabelle: Separate global and local vars in the type environment.

isabelle/core/CoreTyEnv.thy
@@ -20,13 +20,20 @@ record FunInfo =
 
 
 record CoreTyEnv =
-  (* Term-level bindings: variables and constants *)
-  TE_TermVars :: "(string, CoreType) fmap"
+  (* Local variable bindings (mutable or const-local, e.g. let-bindings, function params).
+     These correspond to IS_Locals and IS_Refs in the interpreter state. *)
+  TE_LocalVars :: "(string, CoreType) fmap"
 
-  (* Ghost variables - subset of TE_TermVars keys *)
+  (* Global variable bindings (always constant / read-only).
+     These correspond to IS_Globals in the interpreter state.
+     Globals are implicitly constant and do not appear in TE_ConstNames. *)
+  TE_GlobalVars :: "(string, CoreType) fmap"
+
+  (* Ghost variables - subset of TE_LocalVars and TE_GlobalVars keys *)
   TE_GhostVars :: "string fset"
 
-  (* Constant names - subset of TE_TermVars keys; these are not assignable *)
+  (* Constant local names - subset of TE_LocalVars keys; these are not assignable.
+     Globals are implicitly constant and do not need to appear here. *)
   TE_ConstNames :: "string fset"
 
   (* In-scope type variables (for polymorphic functions) *)
@@ -61,13 +68,27 @@ record CoreTyEnv =
      contains MathInt, MathReal, or another ghost datatype. *)
   TE_GhostDatatypes :: "string fset"
 
+(* Look up a term variable: locals shadow globals *)
+definition tyenv_lookup_var :: "CoreTyEnv \<Rightarrow> string \<Rightarrow> CoreType option" where
+  "tyenv_lookup_var env name =
+    (case fmlookup (TE_LocalVars env) name of
+      Some ty \<Rightarrow> Some ty
+    | None \<Rightarrow> fmlookup (TE_GlobalVars env) name)"
+
+(* A term variable is writable if it is a non-const local.
+   Globals are implicitly constant and never writable. *)
+definition tyenv_var_writable :: "CoreTyEnv \<Rightarrow> string \<Rightarrow> bool" where
+  "tyenv_var_writable env name =
+    (fmlookup (TE_LocalVars env) name \<noteq> None \<and> name |\<notin>| TE_ConstNames env)"
+
 (* tyenv_subset env1 env2: env1 is a "sub-environment" of env2.
    This means env2 has all the same variables (with the same types) plus possibly more.
-   The "fixed" fields (functions, datatypes, return type, type vars) must be identical. *)
+   Only locals may grow; globals and "fixed" fields must be identical. *)
 definition tyenv_subset :: "CoreTyEnv \<Rightarrow> CoreTyEnv \<Rightarrow> bool" where
   "tyenv_subset env1 env2 \<equiv>
-    (\<forall>name ty. fmlookup (TE_TermVars env1) name = Some ty \<longrightarrow>
-               fmlookup (TE_TermVars env2) name = Some ty) \<and>
+    (\<forall>name ty. fmlookup (TE_LocalVars env1) name = Some ty \<longrightarrow>
+               fmlookup (TE_LocalVars env2) name = Some ty) \<and>
+    TE_GlobalVars env1 = TE_GlobalVars env2 \<and>
     TE_GhostVars env1 |\<subseteq>| TE_GhostVars env2 \<and>
     TE_ConstNames env1 |\<subseteq>| TE_ConstNames env2 \<and>
     TE_ReturnType env1 = TE_ReturnType env2 \<and>
@@ -87,5 +108,19 @@ lemma tyenv_subset_trans:
   assumes "tyenv_subset env1 env2" and "tyenv_subset env2 env3"
   shows "tyenv_subset env1 env3"
   using assms unfolding tyenv_subset_def by (auto dest: fsubset_trans)
+
+lemma tyenv_lookup_var_local [simp]:
+  "fmlookup (TE_LocalVars env) name = Some ty \<Longrightarrow> tyenv_lookup_var env name = Some ty"
+  unfolding tyenv_lookup_var_def by simp
+
+lemma tyenv_lookup_var_global:
+  "fmlookup (TE_LocalVars env) name = None \<Longrightarrow>
+   tyenv_lookup_var env name = fmlookup (TE_GlobalVars env) name"
+  unfolding tyenv_lookup_var_def by simp
+
+lemma tyenv_lookup_var_TE_ConstNames_irrelevant [simp]:
+  "tyenv_lookup_var (env \<lparr> TE_ConstNames := c \<rparr>) name = tyenv_lookup_var env name"
+  unfolding tyenv_lookup_var_def by (simp split: option.splits)
+
 
 end
