isabelle/core/CoreTyEnvWellFormed.thy
@@ -2,22 +2,26 @@ theory CoreTyEnvWellFormed
   imports CoreKindcheck
 begin
 
-(* All term variables' types are well-kinded *)
+(* All term variables' types (both local and global) are well-kinded *)
 definition tyenv_vars_well_kinded :: "CoreTyEnv \<Rightarrow> bool" where
   "tyenv_vars_well_kinded env =
-    (\<forall>name ty. fmlookup (TE_TermVars env) name = Some ty \<longrightarrow> is_well_kinded env ty)"
+    ((\<forall>name ty. fmlookup (TE_LocalVars env) name = Some ty \<longrightarrow> is_well_kinded env ty) \<and>
+     (\<forall>name ty. fmlookup (TE_GlobalVars env) name = Some ty \<longrightarrow> is_well_kinded env ty))"
 
 (* All nonghost term variables' types are runtime types *)
 definition tyenv_vars_runtime :: "CoreTyEnv \<Rightarrow> bool" where
   "tyenv_vars_runtime env =
-    (\<forall>name ty. fmlookup (TE_TermVars env) name = Some ty
+    ((\<forall>name ty. fmlookup (TE_LocalVars env) name = Some ty
                \<and> name |\<notin>| TE_GhostVars env
-               \<longrightarrow> is_runtime_type env ty)"
+               \<longrightarrow> is_runtime_type env ty) \<and>
+     (\<forall>name ty. fmlookup (TE_GlobalVars env) name = Some ty
+               \<and> name |\<notin>| TE_GhostVars env
+               \<longrightarrow> is_runtime_type env ty))"
 
-(* Ghost variables are a subset of term variable names *)
+(* Ghost variables are a subset of local and global variable names *)
 definition tyenv_ghost_vars_subset :: "CoreTyEnv \<Rightarrow> bool" where
   "tyenv_ghost_vars_subset env =
-    (TE_GhostVars env |\<subseteq>| fmdom (TE_TermVars env))"
+    (TE_GhostVars env |\<subseteq>| fmdom (TE_LocalVars env) |\<union>| fmdom (TE_GlobalVars env))"
 
 (* The return type is well-kinded *)
 definition tyenv_return_type_well_kinded :: "CoreTyEnv \<Rightarrow> bool" where
@@ -115,14 +119,14 @@ definition tyenv_well_formed :: "CoreTyEnv \<Rightarrow> bool" where
      tyenv_nonghost_payloads_runtime env \<and>
      tyenv_ghost_datatypes_subset env)"
 
-(* Adding a well-kinded, ground, runtime, non-ghost variable preserves tyenv_well_formed. *)
+(* Adding a well-kinded, ground, runtime, non-ghost local variable preserves tyenv_well_formed. *)
 lemma tyenv_well_formed_add_var:
   assumes wf: "tyenv_well_formed env"
     and ty_wk: "is_well_kinded env ty"
     and ty_runtime: "is_runtime_type env ty"
-  shows "tyenv_well_formed (env \<lparr> TE_TermVars := fmupd var ty (TE_TermVars env) \<rparr>)"
+  shows "tyenv_well_formed (env \<lparr> TE_LocalVars := fmupd var ty (TE_LocalVars env) \<rparr>)"
 proof -
-  let ?env' = "env \<lparr> TE_TermVars := fmupd var ty (TE_TermVars env) \<rparr>"
+  let ?env' = "env \<lparr> TE_LocalVars := fmupd var ty (TE_LocalVars env) \<rparr>"
   from wf have wk: "tyenv_vars_well_kinded env"
     and rt: "tyenv_vars_runtime env"
     and gvs: "tyenv_ghost_vars_subset env"
@@ -137,7 +141,7 @@ proof -
               "tyenv_ghost_datatypes_subset env"
     unfolding tyenv_well_formed_def by auto
 
-  \<comment> \<open>is_well_kinded only depends on TE_Datatypes and TE_TypeVars, not TE_TermVars\<close>
+  \<comment> \<open>is_well_kinded only depends on TE_Datatypes and TE_TypeVars, not TE_LocalVars\<close>
   have env'_fields: "TE_TypeVars ?env' = TE_TypeVars env"
                      "TE_Datatypes ?env' = TE_Datatypes env"
     by simp_all
@@ -202,15 +206,15 @@ proof -
   ultimately show ?thesis unfolding tyenv_well_formed_def by auto
 qed
 
-(* Adding a well-kinded ghost variable preserves tyenv_well_formed.
+(* Adding a well-kinded ghost local variable preserves tyenv_well_formed.
    Ghost variables do not need to be runtime types. *)
 lemma tyenv_well_formed_add_ghost_var:
   assumes wf: "tyenv_well_formed env"
     and ty_wk: "is_well_kinded env ty"
-  shows "tyenv_well_formed (env \<lparr> TE_TermVars := fmupd var ty (TE_TermVars env),
+  shows "tyenv_well_formed (env \<lparr> TE_LocalVars := fmupd var ty (TE_LocalVars env),
                                  TE_GhostVars := finsert var (TE_GhostVars env) \<rparr>)"
 proof -
-  let ?env' = "env \<lparr> TE_TermVars := fmupd var ty (TE_TermVars env),
+  let ?env' = "env \<lparr> TE_LocalVars := fmupd var ty (TE_LocalVars env),
                      TE_GhostVars := finsert var (TE_GhostVars env) \<rparr>"
   from wf have wk: "tyenv_vars_well_kinded env"
     and rt: "tyenv_vars_runtime env"
